theories/Dot/typeExtraction.v
@@ -1,0 +1,350 @@
+(** *)
+From stdpp Require Import gmap fin_map_dom.
+From iris.base_logic Require Import invariants.
+From iris.proofmode Require Import tactics.
+
+From D Require Import tactics.
+From D.Dot Require Import dotsyn operational synLemmas unary_lr unary_lr_binding.
+
+Set Primitive Projections.
+Set Implicit Arguments.
+
+Definition stys := gmap stamp ty.
+
+Implicit Types (T: ty) (v: vl) (e: tm) (Γ : ctx) (g: stys) (n: nat) (s: stamp).
+
+Definition gdom {X} (g: gmap stamp X) := dom (gset stamp) g.
+Arguments gdom /.
+
+Definition fresh_stamp {X} (g: gmap stamp X): stamp := fresh (dom (gset stamp) g).
+
+Lemma fresh_stamp_spec {X} (g: gmap stamp X) : fresh_stamp g ∉ gdom g.
+Proof. apply is_fresh. Qed.
+Hint Resolve fresh_stamp_spec.
+
+Lemma ex_fresh_stamp {X} (g: gmap stamp X): { s | s ∉ gdom g }.
+Proof. exists (fresh_stamp g). by apply fresh_stamp_spec. Qed.
+
+Lemma insert_grow g s T: s ∉ gdom g → g ⊆ <[s:=T]> g.
+Proof. intro Hfresh. eapply insert_subseteq, not_elem_of_dom, Hfresh. Qed.
+Hint Resolve insert_grow.
+
+Lemma ex_fresh_stamp_strong g T: { s | s ∉ gdom g ∧ g ⊆ <[s := T]> g }.
+Proof.
+  pose proof (ex_fresh_stamp g) as [s Hfresh].
+  exists s; split; auto.
+Qed.
+
+Lemma ex_fresh_stamp_strong' g T: { s | s ∉ gdom g ∧ gdom g ⊆ gdom (<[s := T]> g) }.
+Proof.
+  pose proof (ex_fresh_stamp_strong g T) as [s []].
+  exists s; split =>//=. by apply subseteq_dom.
+Qed.
+
+(** Next, we define "extraction", which is the core of stamping.
+    Extraction (as defined by [extraction]) is a relation, stable under
+    substitution, between a type and its extracted form.
+
+    An extracted type is basically a stamp pointing into a table, where types
+    are allocated. However, we cannot substitute into such opaque pointers
+    directly, so how can we ensure stability under substitution?
+    To this end, extracted types also contain an environment on which
+    substitution can act.
+    The function [extract] extracts types by allocating them into a table and
+    creating an initial environment.
+ *)
+Definition extractedTy: Type := stamp * vls.
+Definition extractionResult: Type := stys * extractedTy.
+
+Implicit Types (sσ: extractedTy) (gsσ: extractionResult).
+
+Definition extract g n T: stys * extractedTy :=
+  let s := fresh_stamp g
+  in (<[s := T]> g, (s, idsσ n)).
+
+Definition extraction n T: (stys * extractedTy → Prop) :=
+  λ '(g, (s, σ)),
+  ∃ T', g !! s = Some T' ∧ T'.|[to_subst σ] = T ∧ nclosed_σ σ n ∧ nclosed T' (length σ).
+Notation "T ~[ n  ] gsσ" := (extraction n T gsσ) (at level 70).
+
+Lemma extract_spec g n T: nclosed T n → T ~[ n ] (extract g n T).
+Proof. move => Hcl; exists T; by rewrite lookup_insert closed_subst_idsρ ?length_idsσ. Qed.
+Hint Resolve extract_spec.
+
+Lemma nclosed_σ_to_subst ξ σ n:
+  nclosed_σ ξ (length σ) → nclosed_σ σ n →
+  nclosed_σ (ξ.|[to_subst σ]) n.
+Proof.
+  intros.
+  apply closed_vls_to_Forall, fv_to_subst => //. by apply Forall_to_closed_vls.
+Qed.
+Hint Resolve nclosed_σ_to_subst.
+
+Lemma extraction_closed g n T s σ:
+  T ~[ n ] (g, (s, σ)) →
+  nclosed T n.
+Proof. intros (T' & Hlook & <- & Hclσ & HclT'). by apply fv_to_subst. Qed.
+
+Lemma extraction_subst g n T s σ m σ':
+  T ~[ n ] (g, (s, σ)) →
+  length σ' = n →
+  nclosed_σ σ' m →
+  T.|[to_subst σ'] ~[ m ] (g, (s, σ.|[to_subst σ'])).
+Proof.
+  intros (T' & Hlook & <- & Hclσ & HclT') <- => /=. rewrite map_length.
+  exists T'; repeat split => //.
+  - asimpl. apply HclT', to_subst_compose.
+  - by apply nclosed_σ_to_subst.
+Qed.
+Hint Resolve extraction_subst.
+
+Lemma extract_subst_spec g g' n T s σ m σ':
+  nclosed T n →
+  length σ' = n →
+  nclosed_σ σ' m →
+  (g', (s, σ)) = extract g n T →
+  T.|[to_subst σ'] ~[ m ] (g', (s, σ.|[to_subst σ'])).
+Proof.
+  intros * HclT Hlen Hclσ Heq.
+  eapply extraction_subst => //. rewrite Heq. by eapply extract_spec.
+Qed.
+Hint Resolve extract_subst_spec.
+
+Lemma extraction_mono T g g' s σ n:
+  g ⊆ g' →
+  T ~[ n ] (g, (s, σ)) →
+  T ~[ n ] (g', (s, σ)).
+Proof.
+  cbn. intros Hg (T' & Hlook & Heq & ?).
+  exists T'; repeat split => //. by eapply map_subseteq_spec.
+Qed.
+Hint Extern 5 (_ ~[ _ ] (_, _)) => try_once extraction_mono.
+
+Lemma extract_spec_growg g n T g' sσ:
+  (g', sσ) = extract g n T → g ⊆ g'.
+Proof.
+  intros H; cinject H. apply insert_grow, fresh_stamp_spec.
+Qed.
+Hint Resolve extract_spec_growg.
+
+Lemma lookup_mono g g' s T:
+  g !! s = Some T →
+  g ⊆ g' →
+  g' !! s = Some T.
+Proof.
+  intros Hlook Hless. pose proof (Hless s) as H.
+  rewrite Hlook /= in H; by (case_match; subst).
+Qed.
+Hint Extern 5 (_ !! _ = Some _) => try_once lookup_mono.
+
+Hint Resolve @fv_to_subst fv_to_subst_vl.
+
+Lemma extract_lookup g g' s σ n T:
+  (g', (s, σ)) = extract g n T → g' !! s = Some T.
+Proof. intros H; cinject H; by rewrite lookup_insert. Qed.
+Hint Resolve extract_lookup.
+
+Lemma extraction_lookup g s σ n T:
+  T ~[ n ] (g, (s, σ)) → ∃ T', g !! s = Some T' ∧ T'.|[to_subst σ] = T.
+Proof. naive_solver. Qed.
+
+Lemma subst_compose_extract g g' T n m ξ σ s:
+  nclosed T n →
+  nclosed_σ ξ m →
+  length ξ = n →
+  (g', (s, σ)) = extract g n T →
+  T.|[to_subst σ.|[to_subst ξ]] = T.|[to_subst σ].|[to_subst ξ].
+Proof.
+  intros HclT Hclξ Hlen Hext; cinject Hext. by eapply subst_compose_idsσ_x.
+Qed.
+
+Lemma extract_subst_commute g g' g'' T ξ n m s1 σ1 s2 σ2:
+  nclosed T n →
+  nclosed_σ ξ m →
+  length ξ = n →
+  (g', (s1, σ1)) = extract g n T →
+  (g'', (s2, σ2)) = extract g' m (T.|[to_subst ξ]) →
+  T.|[to_subst ξ] ~[ m ] (g'', (s1, σ1.|[to_subst ξ])) ∧
+  ∃ T1 T2,
+    g'' !! s1 = Some T1 ∧
+    g'' !! s2 = Some T2 ∧
+    (* T1.|[to_subst σ1].|[to_subst ξ] = T2.|[to_subst σ2]. *)
+    T1.|[to_subst σ1.|[to_subst ξ]] = T2.|[to_subst σ2].
+Proof.
+  intros HclT Hclξ Hlen Hext1 Hext2. split; eauto.
+  exists T, T.|[to_subst ξ]; split_and!; eauto.
+  (* - apply (@lookup_mono g' g''); info_eauto. *)
+  (*   cinject Hext1; by rewrite lookup_insert. *)
+  (* - cinject Hext2; by rewrite lookup_insert. *)
+  - erewrite subst_compose_extract => //.
+    cinject Hext1; cinject Hext2.
+    rewrite !closed_subst_idsρ => //.
+    apply fv_to_subst; eauto. (* eauto with typeclass_instances. *)
+Qed.
+
+Section interp_equiv.
+  Context `{!dotG Σ}.
+
+  Notation envD := (listVlC -n> vlC -n> iProp Σ).
+  Implicit Types (φ: envD).
+
+  (** This interpretation is too naive: it substitutes σ into T' *before* applying our semantics,
+      but we will not be able to do this when we use saved propositions to pre-interpret T'. *)
+  Definition interp_extractedTy_naive: extractionResult -> envD :=
+    λ gsσ, λne ρ v,
+    let '(g, (s, σ)) := gsσ in
+    (∃ T' : ty, ⌜g !! s = Some T'⌝ ∧ ⟦ T'.|[to_subst σ] ⟧ ρ v)%I.
+
+  (** We can relate the  ⟦ T ⟧ with the naive stamp semantics at all environments. *)
+  Lemma extraction_envD_equiv_naive g s σ T n ρ v:
+    T ~[ n ] (g, (s, σ)) →
+    (⟦ T ⟧ ρ v ↔ interp_extractedTy_naive (g, (s, σ)) ρ v)%I.
+  Proof.
+    cbn; intros (T' & -> & <- & HclT & HclT').
+    iSplit; iIntros "H"; [| iDestruct "H" as (T'' Heq) "?" ]; naive_solver.
+  Qed.
+
+  (** However, a stamp semantics that carries over to saved predicates must use
+      σ in ρ. And the result is only equivalent for closed ρ with the expected length. *)
+  Definition interp_extractedTy: (ty * vls) → envD :=
+    λ '(T, σ), λne ρ v,
+    (⟦ T ⟧ (subst_sigma σ ρ) v)%I.
+  Notation "⟦ T ⟧ [ σ ]" := (interp_extractedTy (T, σ)).
+
+  Definition envD_equiv n φ1 φ2: iProp Σ :=
+    (∀ ρ v, ⌜ length ρ = n ⌝ → ⌜ cl_ρ ρ ⌝ → φ1 ρ v ≡ φ2 ρ v)%I.
+  Notation "φ1 ≈[  n  ] φ2" := (envD_equiv n φ1 φ2) (at level 70).
+
+  (* Belongs in synLemmas. *)
+  Lemma interp_subst_commute T σ ρ v:
+    nclosed T (length σ) →
+    nclosed_σ σ (length ρ) →
+    cl_ρ ρ →
+    ⟦ T.|[to_subst σ] ⟧ ρ v ≡ ⟦ T ⟧ σ.|[to_subst ρ] v.
+  Proof.
+    intros HclT Hclσ Hclρ.
+    rewrite -(interp_subst_all ρ _ v) // -(interp_subst_all _ T v).
+    - by erewrite subst_compose_x.
+    - by apply nclosed_σ_to_subst.
+  Qed.
+
+  Lemma extraction_envD_equiv g s σ T n:
+    T ~[ n ] (g, (s, σ)) →
+    (∃ T', ⌜ g !! s = Some T'⌝ ∧
+        ⟦ T ⟧ ≈[ n ] ⟦ T' ⟧ [ σ ])%I.
+  Proof.
+    iIntros ((T' & -> & <- & HclT & HclT')). iExists _; iSplit => //.
+    iIntros (ρ v <- Hclρ). by rewrite interp_subst_commute /subst_sigma.
+  Qed.
+
+  (** envD_equiv commutes with substitution. *)
+  Lemma envD_equiv_subst g T m n ξ s1 σ1 s2 σ2:
+    T ~[ m ] (g, (s1, σ1)) →
+    T.|[to_subst ξ] ~[ n ] (g, (s2, σ2)) →
+    length ξ = m →
+    nclosed_σ ξ n →
+    (∃ T1 T2, ⌜ g !! s1 = Some T1⌝ ∧ ⌜ g !! s2 = Some T2 ⌝ ∧
+    ⟦ T1 ⟧ [ σ1.|[to_subst ξ] ] ≈[ n ] ⟦ T2 ⟧ [ σ2 ])%I.
+  Proof.
+    rewrite /interp_extractedTy; iIntros ((T1 & -> & Heq1 & Hclσ1 & HclT1) (T2 & -> & Heq2 & Hclσ2 & HclT2) Hlenξ Hclξ).
+    iExists _, _; repeat iSplit => //; iIntros (ρ v Hlenρ Hclρ) "/="; subst.
+    assert (Hclσ1ξ: nclosed_σ σ1.|[to_subst ξ] (length ρ)). by apply nclosed_σ_to_subst.
+    assert (Hrew: T2.|[to_subst σ2.|[to_subst ρ]] =
+                  T1.|[to_subst σ1.|[to_subst ξ].|[to_subst ρ]]). by repeat erewrite subst_compose_x;
+                                                                    rewrite ?map_length ?Heq1 ?Heq2.
+    rewrite -(interp_subst_all _ T1) -?(interp_subst_all _ T2) ?Hrew //; by apply nclosed_σ_to_subst.
+  Qed.
+
+  Notation "¬ P" := (□ (P → False))%I : bi_scope.
+
+
+  Notation "s ↦ γ" := (mapsto (hG := dotG_interpNames) s γ)  (at level 20) : bi_scope.
+                           (* (◯ {[ s := to_agree (γ : leibnizC gname) ]})) *)
+  Global Instance: Persistent (s ↦ γ).
+  Proof. apply _. Qed.
+  Global Instance: Timeless (s ↦ γ).
+  Proof. apply _. Qed.
+
+  Notation "s ↝ φ" := (∃ γ, s ↦ γ ∗ γ ⤇ (λ (vs: vls) v, φ vs v))%I  (at level 20) : bi_scope.
+
+  Definition allGs gs := (gen_iheap_ctx (hG := dsubG_interpNames) gs).
+  Arguments allGs /.
+
+  Lemma alloc_sp T: (|==> ∃ γ, γ ⤇ dsub_interp T)%I.
+  Proof. by apply saved_interp_alloc. Qed.
+
+  Lemma transferOne_base_inv gs s T:
+      gs !! s = None → (allGs gs ==∗ ∃ gs', allGs gs' ∗ s ↝ ⟦ T ⟧ ∗ ⌜ gdom gs' ≡ gdom gs ∪ {[s]} ⌝)%I.
+  Proof.
+    iIntros (HsFresh) "Hown /=".
+    iMod (alloc_sp T) as (γ) "#Hγ".
+    iMod (gen_iheap_alloc _ s γ with "Hown") as "[H1 H2]" => //.
+    iModIntro. iExists (<[s:=γ]> gs). iFrame. iSplitL.
+    - iExists γ. by iFrame.
+    - by rewrite dom_insert union_comm.
+  Qed.
+
+  (* To give a definitive version of wellMapped, we need stampHeap to be stored in a resource. Here it is: *)
+  Definition wellMapped g : iProp Σ :=
+    (□∀ s T ρ v,
+        ⌜ g !! s = Some T⌝ → ∃ φ, s ↝ φ ∧ ⟦ T ⟧ ρ v ≡ φ ρ v)%I.
+  Instance: Persistent (wellMapped g).
+  Proof. apply _. Qed.
+
+  (** We can transfer one mapping from [g] into Iris resources. Note that [gs ⊆
+      gs'] in the outpu might not be ultimately needed; that's enforced indirectly
+      by both wellMapped and by invariants. *)
+  Lemma transferOne gs g s T:
+      gs !! s = None → (wellMapped g → allGs gs ==∗ ∃ gs', wellMapped (<[s := T]> g) ∧ allGs gs' ∧ ⌜gdom gs' ≡ gdom gs ∪ {[s]}⌝)%I.
+  Proof.
+    iIntros (HsFresh) "#Hg Hown /=".
+    iMod (transferOne_base_inv gs s T HsFresh with "Hown") as (gs') "(Hgs & #Hmaps & #Hdom)".
+    iExists gs'; iModIntro; iFrame "Hgs".
+    iSplit =>//.
+    iIntros (s' T' ρ v Hlook) "!>".
+    destruct (decide (s = s')) as [<-|Hne].
+    - iExists (⟦ T ⟧).
+      suff <-: T = T' by iSplit. rewrite lookup_insert in Hlook; by injection Hlook.
+    - rewrite lookup_insert_ne //= in Hlook. by iApply "Hg".
+  Qed.
+
+  Lemma transfer' g gs: (∀ s, s ∈ gdom g → gs !! s = None) →
+                       (allGs gs ==∗ ∃ gs', wellMapped g ∧ allGs gs' ∧ ⌜gdom gs' ≡ gdom gs ∪ gdom g⌝).
+  Proof.
+    elim g using map_ind.
+    - iIntros "/=" (H) "Hgs !>". iExists gs. repeat iSplit => //.
+      + by iIntros (?????).
+      + iPureIntro. rewrite dom_empty. set_solver.
+    - move=> {g} /=. iIntros (s T g Hs IH Hdom) "Hallgs".
+      setoid_rewrite dom_insert in Hdom.
+      iPoseProof (IH with "Hallgs") as "IH".
+      { move=> s' Hs'. apply Hdom. set_solver. }
+      iMod "IH" as (gs') "[Hwm [Hgs %]]". move: H => Hgs'.
+
+      iPoseProof (transferOne gs' g s T) as "HH".
+      + cut (s ∉ dom (gset stamp) gs').
+        * move=> Hsgs. by eapply not_elem_of_dom.
+        * rewrite Hgs'. apply not_elem_of_union.
+          split; eapply not_elem_of_dom =>//. apply Hdom. set_solver.
+      + iMod ("HH" with "Hwm Hgs") as (gs'') "[H1 [H2 %]]". move: H => /= Hgs''.
+        iExists gs''. iFrame; iPureIntro.
+        rewrite dom_insert Hgs'' Hgs'. (* set_solver very slow, so: *)
+        (* clear; set_solver. (* 0.2 s *) *)
+        by rewrite -union_assoc [dom _ _ ∪ {[_]}]union_comm.
+  Qed.
+
+  Lemma transfer g gs: (∀ s, s ∈ gdom g → gs !! s = None) →
+                       (allGs gs ==∗ wellMapped g)%I.
+  Proof.
+    iIntros (Hs) "H". by iMod (transfer' gs Hs with "H") as (gs') "[H ?]".
+  Qed.
+
+  Lemma leadsto_agree s φ1 φ2 ρ v: s ↝ φ1 -∗ s ↝ φ2 -∗ ▷ (φ1 ρ v ≡ φ2 ρ v).
+  Proof.
+    iIntros "/= #H1 #H2".
+    iDestruct "H1" as (γ1) "[Hs1 Hg1]".
+    iDestruct "H2" as (γ2) "[Hs2 Hg2]".
+    iPoseProof (mapsto_agree with "Hs1 Hs2") as "%"; subst.
+    by iApply (saved_interp_agree_eta _ φ1 φ2).
+  Qed.
+End interp_equiv.
